ulib/FStar.ListProperties.fst
@@ -60,34 +60,34 @@ let rev_mem #a l x = rev_acc_mem l [] x
 
 (** Properties about append **)
 
-val append_nil_l: #a:eqtype -> l:list a ->
+val append_nil_l: l:list 'a ->
   Lemma (requires True)
-        (ensures ([]@l = l))
-let append_nil_l #a l = ()
+        (ensures ([]@l == l))
+let append_nil_l l = ()
 
-val append_l_nil: #a:eqtype -> l:list a ->
+val append_l_nil: l:list 'a ->
   Lemma (requires True)
-        (ensures (l@[] = l)) [SMTPat (l@[])]
-let rec append_l_nil #a = function
+        (ensures (l@[] == l)) [SMTPat (l@[])]
+let rec append_l_nil = function
   | [] -> ()
   | hd::tl -> append_l_nil tl
 
-val append_cons_l: #a:eqtype -> hd:a -> tl:list a -> l:list a ->
+val append_cons_l: hd:'a -> tl:list 'a -> l:list 'a ->
   Lemma (requires True)
-        (ensures (((hd::tl)@l) = (hd::(tl@l))))
-let append_cons_l #a hd tl l = ()
+        (ensures (((hd::tl)@l) == (hd::(tl@l))))
+let append_cons_l hd tl l = ()
 
-val append_l_cons: #a:eqtype -> hd:a -> tl:list a -> l:list a ->
+val append_l_cons: hd:'a -> tl:list 'a -> l:list 'a ->
   Lemma (requires True)
-        (ensures ((l@(hd::tl)) = ((l@[hd])@tl)))
-let rec append_l_cons #a hd tl l = match l with
+        (ensures ((l@(hd::tl)) == ((l@[hd])@tl)))
+let rec append_l_cons hd tl l = match l with
     | [] -> ()
     | hd'::tl' -> append_l_cons hd tl tl'
 
-val append_assoc: #a:eqtype -> l1:list a -> l2:list a -> l3:list a ->
+val append_assoc: l1:list 'a -> l2:list 'a -> l3:list 'a ->
   Lemma (requires True)
-        (ensures ((l1@(l2@l3)) = ((l1@l2)@l3)))
-let rec append_assoc #a l1 l2 l3 = match l1 with
+        (ensures ((l1@(l2@l3)) == ((l1@l2)@l3)))
+let rec append_assoc l1 l2 l3 = match l1 with
     | [] -> ()
     | hd::tl -> append_assoc tl l2 l3
 
@@ -134,27 +134,27 @@ let rec append_count_forall #a l1 l2 = match l1 with
   | [] -> ()
   | hd::tl -> append_count_forall tl l2
 
-val append_eq_nil: #a:eqtype -> l1:list a -> l2:list a ->
-  Lemma (requires (l1@l2 = []))
-        (ensures (l1 = [] /\ l2 = []))
-let append_eq_nil #a l1 l2 = ()
+val append_eq_nil: l1:list 'a -> l2:list 'a ->
+  Lemma (requires (l1@l2 == []))
+        (ensures (l1 == [] /\ l2 == []))
+let append_eq_nil l1 l2 = ()
 
-val append_eq_singl: #a:eqtype -> l1:list a -> l2:list a -> x:a ->
-  Lemma (requires (l1@l2 = [x]))
-        (ensures ((l1 = [x] /\ l2 = []) \/ (l1 = [] /\ l2 = [x])))
-let append_eq_singl #a l1 l2 x = ()
+val append_eq_singl: l1:list 'a -> l2:list 'a -> x:'a ->
+  Lemma (requires (l1@l2 == [x]))
+        (ensures ((l1 == [x] /\ l2 == []) \/ (l1 == [] /\ l2 == [x])))
+let append_eq_singl l1 l2 x = ()
 
-val append_inv_head: #a:eqtype -> l:list a -> l1:list a -> l2:list a ->
-  Lemma (requires ((l@l1) = (l@l2)))
-        (ensures (l1 = l2))
-let rec append_inv_head #a l l1 l2 = match l with
+val append_inv_head: l:list 'a -> l1:list 'a -> l2:list 'a ->
+  Lemma (requires ((l@l1) == (l@l2)))
+        (ensures (l1 == l2))
+let rec append_inv_head l l1 l2 = match l with
     | [] -> ()
     | hd::tl -> append_inv_head tl l1 l2
 
-val append_inv_tail: #a:eqtype -> l:list a -> l1:list a -> l2:list a ->
-  Lemma (requires ((l1@l) = (l2@l)))
-        (ensures (l1 = l2))
-let rec append_inv_tail #a l l1 l2 = match l1, l2 with
+val append_inv_tail: l:list 'a -> l1:list 'a -> l2:list 'a ->
+  Lemma (requires ((l1@l) == (l2@l)))
+        (ensures (l1 == l2))
+let rec append_inv_tail l l1 l2 = match l1, l2 with
     | [], [] -> ()
     | hd1::tl1, hd2::tl2 -> append_inv_tail l tl1 tl2
     | [], hd2::tl2 ->
@@ -179,41 +179,41 @@ let rec rev' = function
   | hd::tl -> (rev' tl)@[hd]
 let rev'T = rev'
 
-val rev_acc_rev': #a:eqtype -> l:list a -> acc:list a ->
+val rev_acc_rev': l:list 'a -> acc:list 'a ->
   Lemma (requires (True))
-        (ensures ((rev_acc l acc) = ((rev' l)@acc)))
-let rec rev_acc_rev' #a l acc = match l with
+        (ensures ((rev_acc l acc) == ((rev' l)@acc)))
+let rec rev_acc_rev' l acc = match l with
     | [] -> ()
     | hd::tl -> rev_acc_rev' tl (hd::acc); append_l_cons hd acc (rev' tl)
 
-val rev_rev': #a:eqtype -> l:list a ->
+val rev_rev': l:list 'a ->
   Lemma (requires True)
-        (ensures ((rev l) = (rev' l)))
-let rev_rev' #a l = rev_acc_rev' l []; append_l_nil (rev' l)
+        (ensures ((rev l) == (rev' l)))
+let rev_rev' l = rev_acc_rev' l []; append_l_nil (rev' l)
 
-val rev'_append: #a:eqtype -> l1:list a -> l2:list a ->
+val rev'_append: l1:list 'a -> l2:list 'a ->
   Lemma (requires True)
-        (ensures ((rev' (l1@l2)) = ((rev' l2)@(rev' l1))))
-let rec rev'_append #a l1 l2 = match l1 with
+        (ensures ((rev' (l1@l2)) == ((rev' l2)@(rev' l1))))
+let rec rev'_append l1 l2 = match l1 with
     | [] -> append_l_nil (rev' l2)
     | hd::tl -> rev'_append tl l2; append_assoc (rev' l2) (rev' tl) [hd]
 
-val rev_append: #a:eqtype -> l1:list a -> l2:list a ->
+val rev_append: l1:list 'a -> l2:list 'a ->
   Lemma (requires True)
-        (ensures ((rev (l1@l2)) = ((rev l2)@(rev l1))))
-let rev_append #a l1 l2 = rev_rev' l1; rev_rev' l2; rev_rev' (l1@l2); rev'_append l1 l2
+        (ensures ((rev (l1@l2)) == ((rev l2)@(rev l1))))
+let rev_append l1 l2 = rev_rev' l1; rev_rev' l2; rev_rev' (l1@l2); rev'_append l1 l2
 
-val rev'_involutive : #a:eqtype -> l:list a ->
+val rev'_involutive : l:list 'a ->
   Lemma (requires True)
-        (ensures (rev' (rev' l) = l))
-let rec rev'_involutive #a = function
+        (ensures (rev' (rev' l) == l))
+let rec rev'_involutive = function
   | [] -> ()
   | hd::tl -> rev'_append (rev' tl) [hd]; rev'_involutive tl
 
-val rev_involutive : #a:eqtype -> l:list a ->
+val rev_involutive : l:list 'a ->
   Lemma (requires True)
-        (ensures (rev (rev l) = l))
-let rev_involutive #a l = rev_rev' l; rev_rev' (rev' l); rev'_involutive l
+        (ensures (rev (rev l) == l))
+let rev_involutive l = rev_rev' l; rev_rev' (rev' l); rev'_involutive l
 
 
 (** Reverse induction principle **)
@@ -225,10 +225,10 @@ let rec rev'_list_ind p = function
   | [] -> ()
   | hd::tl -> rev'_list_ind p tl
 
-val rev_ind: #a:eqtype -> p:(list a -> Tot bool) -> l:list a ->
+val rev_ind: p:(list 'a -> Tot bool) -> l:list 'a ->
   Lemma (requires ((p []) /\ (forall hd tl. p hd ==> p (hd@[tl]))))
         (ensures (p l))
-let rev_ind #a p l = rev'_involutive l; rev'_list_ind p (rev' l)
+let rev_ind p l = rev'_involutive l; rev'_list_ind p (rev' l)
 
 (** Properties about iterators **)
 
@@ -312,9 +312,9 @@ let rec sorted f = function
   | [_] -> true
   | x::y::tl -> f x y && sorted f (y::tl)
 
-type total_order (#a:eqtype) (f: (a -> a -> Tot bool)) =
+type total_order (#a:Type) (f: (a -> a -> Tot bool)) =
     (forall a. f a a)                                           (* reflexivity   *)
-    /\ (forall a1 a2. f a1 a2 /\ f a2 a1  ==> a1 = a2)          (* anti-symmetry *)
+    /\ (forall a1 a2. f a1 a2 /\ f a2 a1  ==> a1 == a2)          (* anti-symmetry *)
     /\ (forall a1 a2 a3. f a1 a2 /\ f a2 a3 ==> f a1 a3)        (* transitivity  *)
     /\ (forall a1 a2. f a1 a2 \/ f a2 a1)                       (* totality *)
 
